src/Reduction.v
@@ -1,0 +1,65 @@
+Require Import Bool List String Peano_dec.
+Require Import Common ListSupport FMap Syntax Semantics StepT SemFacts.
+
+Definition NonSilentHistory (hst: THistory) :=
+  Forall (fun tlbl => tlbl <> emptyRLabel) hst.
+
+Definition NotMsgIn {MsgT} (lbl: RLabel MsgT) :=
+  match lbl with
+  | RlblIn _ => False
+  | _ => True
+  end.
+
+Definition NonMsgInHistory (hst: THistory) :=
+  Forall (fun tlbl => NotMsgIn tlbl) hst.
+
+Lemma msg_in_commutes:
+  forall sys st1 emsg tlbl st2,
+    NotMsgIn tlbl ->
+    steps step_t sys st1 [RlblIn emsg; tlbl] st2 ->
+    steps step_t sys st1 [tlbl; RlblIn emsg] st2.
+Proof.
+  intros.
+  destruct tlbl as [|hdl mins mouts]; [elim H|].
+  repeat match goal with
+         | [H: steps step_t sys _ _ _ |- _] => inv H
+         | [H: step_t sys _ _ _ |- _] => inv H
+         end.
+  - repeat econstructor; eauto.
+  - econstructor.
+    + repeat econstructor; eauto.
+    + inv H7.
+Admitted.
+
+Lemma msg_in_reduced:
+  forall sys st1 emsg hst2 st2,
+    steps step_t sys st1 (RlblIn emsg :: hst2) st2 ->
+    NonMsgInHistory hst2 ->
+    steps step_t sys st1 (hst2 ++ [RlblIn emsg]) st2.
+Proof.
+  induction hst2 as [|tlbl ?]; intros; [assumption|].
+
+  inv H0.
+  change (RlblIn emsg :: tlbl :: hst2) with ([RlblIn emsg; tlbl] ++ hst2) in H.
+  eapply steps_split in H; [|reflexivity].
+  destruct H as [sti [? ?]].
+  apply msg_in_commutes in H0; auto.
+  pose proof (steps_append H H0); clear H H0.
+  simpl in H1; inv H1.
+  specialize (IHhst2 _ H5 H4).
+  simpl; econstructor; eassumption.
+Qed.
+
+Lemma msg_in_reduced_app:
+  forall sys st1 hst1 emsg hst2 st2,
+    steps step_t sys st1 (hst1 ++ RlblIn emsg :: hst2) st2 ->
+    NonMsgInHistory hst2 ->
+    steps step_t sys st1 (hst1 ++ hst2 ++ [RlblIn emsg]) st2.
+Proof.
+  intros.
+  eapply steps_split in H; [|reflexivity].
+  destruct H as [sti [? ?]].
+  apply msg_in_reduced in H; auto.
+  eapply steps_append; eauto.
+Qed.
+
